examples/pseudo_bool/pb_parseScript.sml
@@ -105,6 +105,12 @@ Definition print_annot_prob_def:
     obstr ++ presstr ++ MAP annot_pbc_string fml
 End
 
+(* Multi-objective problem: one min: line per objective, then the constraints *)
+Definition print_mo_prob_def:
+  print_mo_prob (objs,fml) =
+  MAP obj_string objs ++ MAP pbc_string fml
+End
+
 (* Strips annotations *)
 Definition strip_annot_prob_def:
   strip_annot_prob (pres,obj,afml) =
@@ -491,6 +497,30 @@ End
 (* Parse a list of strings in annotated pbf format *)
 Definition parse_pbf_def:
   parse_pbf strs = parse_pbf_toks (MAP toks strs)
+End
+
+(* parse a run of objective lines *)
+Definition parse_objs_maybe_def:
+  (parse_objs_maybe [] acc = (REVERSE acc, [])) ∧
+  (parse_objs_maybe (l::ls) acc =
+  case parse_obj l of
+    NONE => (REVERSE acc, l::ls)
+  | SOME obj => parse_objs_maybe ls (obj::acc))
+End
+
+(* Parse the tokenized multi-objective pbf file *)
+Definition parse_mo_pbf_toks_def:
+  parse_mo_pbf_toks tokss =
+  let nocomments = FILTER nocomment_line tokss in
+  let (objs,rest) = parse_objs_maybe nocomments [] in
+  case parse_constraints rest [] of
+    NONE => NONE
+  | SOME pbf => SOME (objs, MAP SND pbf)
+End
+
+(* Parse a list of strings in multi-objective pbf format *)
+Definition parse_mo_pbf_def:
+  parse_mo_pbf strs = parse_mo_pbf_toks (MAP toks strs)
 End
 
 (*
