examples/pseudo_bool/array/compilation/npbc_mo_fullCompileScript.sml
@@ -1,0 +1,14 @@
+(*
+  Compiles the multi-objective PB checker by evaluation inside the logic of HOL
+*)
+Theory npbc_mo_fullCompile
+Ancestors
+  npbc_mo_fullProg
+Libs
+  preamble eval_cake_compile_x64Lib eval_cake_compile_arm8Lib
+
+Theorem npbc_mo_full_compiled =
+  eval_cake_compile_x64 "" main_prog_def "cake_pb_mo.S";
+
+Theorem npbc_mo_full_compiled_arm8 =
+  eval_cake_compile_arm8 "arm8_" main_prog_def "cake_pb_mo_arm8.S";
