examples/pseudo_bool/array/npbc_mo_fullProgScript.sml
@@ -1,0 +1,432 @@
+(*
+  Multi-objective OPB frontend: parse an OPB file with several objectives,
+  then either print it back or check a PB proof of its nondominated set
+*)
+Theory npbc_mo_fullProg
+Ancestors
+  basis_ffi pb_parse pbc_mo pbc_normalise npbc_parseProg npbc_mo_arrayProg
+Libs
+  preamble basis
+
+val _ = translation_extends"npbc_mo_arrayProg";
+
+(* Translation for parsing a multi-objective OPB file *)
+val r = translate nocomment_line_def;
+
+val r = translate parse_constraint_def;
+val r = translate parse_annot_def;
+val r = translate parse_annot_constraint_def;
+val r = translate parse_constraints_def;
+
+val r = translate parse_obj_def;
+val r = translate parse_objs_maybe_def;
+val r = translate parse_mo_pbf_toks_def;
+
+Definition noparse_string_def:
+  noparse_string f s = concat[«c Input file: »;f;« unable to parse in format: »; s;«\n»]
+End
+
+val r = translate noparse_string_def;
+
+Quote add_cakeml:
+  fun parse_mo_pbf_full f =
+  (case TextIO.inputAllTokensFile #"\n" f blanks tokenize of
+    None => Inl (notfound_string f)
+  | Some lines =>
+  (case parse_mo_pbf_toks lines of
+    None => Inl (noparse_string f "OPB")
+  | Some res => Inr res
+  ))
+End
+
+val inputAllTokensFile_spec_specialize =
+  inputAllTokensFile_spec
+  |> Q.GEN `f` |> Q.SPEC`blanks`
+  |> Q.GEN `fv` |> Q.SPEC`blanks_v`
+  |> Q.GEN `g` |> Q.ISPEC`tokenize`
+  |> Q.GEN `gv` |> Q.ISPEC`tokenize_v`
+  |> Q.GEN `a` |> Q.ISPEC`SUM_TYPE STRING_TYPE INT`
+  |> REWRITE_RULE [blanks_v_thm,tokenize_v_thm] ;
+
+Definition get_mo_fml_def:
+  get_mo_fml fs f =
+  if inFS_fname fs f then
+    parse_mo_pbf (all_lines_file fs f)
+  else NONE
+End
+
+Theorem parse_mo_pbf_full_spec:
+  STRING_TYPE f fv ∧
+  validArg f ∧
+  hasFreeFD fs
+  ⇒
+  app (p:'ffi ffi_proj) ^(fetch_v"parse_mo_pbf_full"(get_ml_prog_state()))
+    [fv]
+    (STDIO fs)
+    (POSTv v.
+    & (∃err. (SUM_TYPE STRING_TYPE mo_prob_TYPE)
+    (case get_mo_fml fs f of
+      NONE => INL err
+    | SOME res => INR res) v) * STDIO fs)
+Proof
+  rw[]>>
+  xcf"parse_mo_pbf_full"(get_ml_prog_state())>>
+  reverse (Cases_on `STD_streams fs`) >- (fs [TextIOProofTheory.STDIO_def] \\ xpull) >>
+  reverse (Cases_on`consistentFS fs`) >- (
+    fs [STDIO_def,IOFS_def,wfFS_def,consistentFS_def]
+    \\ xpull \\ metis_tac[]) >>
+  xlet`(POSTv sv. &OPTION_TYPE (LIST_TYPE (LIST_TYPE (SUM_TYPE STRING_TYPE INT)))
+            (if inFS_fname fs f then
+               SOME(MAP (MAP tokenize o tokens blanks) (all_lines_file fs f))
+             else NONE) sv * STDIO fs)`
+  >- (
+    xapp_spec inputAllTokensFile_spec_specialize >>
+    xsimpl>>
+    simp[pb_parseTheory.blanks_def]>>
+    fs[FILENAME_def,validArg_def,blanks_v_thm]>>
+    first_x_assum (irule_at Any)>>
+    first_x_assum (irule_at Any)>>
+    first_x_assum (irule_at Any)>>
+    qexists_tac`emp`>>xsimpl)>>
+  simp[get_mo_fml_def]>>
+  IF_CASES_TAC>>fs[OPTION_TYPE_def]>>xmatch
+  >- (
+    xlet_autop>>
+    `toks = (MAP tokenize ∘ tokens blanks)` by
+      metis_tac[toks_def,ETA_AX,o_DEF]>>
+    rw[parse_mo_pbf_def]>>
+    qmatch_goalsub_abbrev_tac`option_CASE AAA`>>
+    Cases_on`AAA`>>
+    fs[OPTION_TYPE_def]
+    >- (
+      xmatch >>
+      xlet_autop>>
+      xcon>>xsimpl>>
+      simp[SUM_TYPE_def]>>metis_tac[])>>
+    xmatch>>
+    xcon>>
+    xsimpl>>
+    simp[SUM_TYPE_def])>>
+  xlet_autop>>
+  xcon>>xsimpl>>
+  simp[SUM_TYPE_def]>>metis_tac[]
+QED
+
+Definition check_unsat_2_sem_def:
+  check_unsat_2_sem fs f1 out ⇔
+  case get_mo_fml fs f1 of
+    SOME mprob => out = concat (print_mo_prob mprob)
+  | NONE => out = «»
+End
+
+Quote add_cakeml:
+  fun check_unsat_2 f1 =
+  case parse_mo_pbf_full f1 of
+    Inl err => TextIO.output TextIO.stdErr err
+  | Inr mprob =>
+    TextIO.print_list (print_mo_prob mprob)
+End
+
+Theorem check_unsat_2_spec:
+  STRING_TYPE f1 f1v ∧ validArg f1 ∧
+  hasFreeFD fs
+  ⇒
+  app (p:'ffi ffi_proj) ^(fetch_v"check_unsat_2"(get_ml_prog_state()))
+    [f1v]
+    (STDIO fs)
+    (POSTv uv. &UNIT_TYPE () uv *
+    SEP_EXISTS out err.
+      STDIO (add_stdout (add_stderr fs err) out) *
+      &(check_unsat_2_sem fs f1 out))
+Proof
+  rw[check_unsat_2_sem_def]>>
+  xcf "check_unsat_2" (get_ml_prog_state ())>>
+  reverse (Cases_on `STD_streams fs`) >- (fs [TextIOProofTheory.STDIO_def] \\ xpull) >>
+  xlet_autop>>
+  pop_assum mp_tac>>
+  TOP_CASE_TAC
+  >- (
+    simp[SUM_TYPE_def]>>rw[]>>
+    xmatch>>
+    xapp_spec output_stderr_spec \\ xsimpl>>
+    asm_exists_tac>>xsimpl>>
+    qexists_tac`emp`>>xsimpl>>
+    qexists_tac`fs`>>xsimpl>>
+    rw[]>>
+    qexists_tac`err`>>xsimpl>>rw[]>>
+    fs[STD_streams_add_stderr, STD_streams_stdout,add_stdo_nil]>>
+    xsimpl)>>
+  simp[SUM_TYPE_def]>>rw[]>>
+  xmatch>>
+  xlet_autop>>
+  xapp_spec print_list_spec>>xsimpl>>
+  asm_exists_tac>>xsimpl>>
+  qexists_tac`emp`>>qexists_tac`fs`>>xsimpl>>
+  rw[]>>
+  qexists_tac`«»`>>
+  simp[STD_streams_stderr,add_stdo_nil]>>
+  xsimpl
+QED
+
+Definition check_unsat_3_sem_def:
+  check_unsat_3_sem fs ord f1 out ⇔
+  (out ≠ «» ⇒
+  ∃objs fml vs.
+    get_mo_fml fs f1 = SOME (objs,fml) ∧
+    out = print_front_str ord vs ∧
+    set vs = pbc_mo$nondom_set ord (set fml) objs)
+End
+
+Quote add_cakeml:
+  fun check_unsat_3 ord f1 f2 =
+  case parse_mo_pbf_full f1 of
+    Inl err => TextIO.output TextIO.stdErr err
+  | Inr mprob =>
+    (case map_front_to_string ord (check_unsat_mo_top_norm ord mprob f2) of
+      Inl err => TextIO.output TextIO.stdErr err
+    | Inr s => TextIO.print s)
+End
+
+Theorem check_unsat_3_spec:
+  PBC_MO_MO_ORD_TYPE ord ordv ∧
+  STRING_TYPE f1 f1v ∧ validArg f1 ∧
+  STRING_TYPE f2 f2v ∧ validArg f2 ∧
+  hasFreeFD fs
+  ⇒
+  app (p:'ffi ffi_proj) ^(fetch_v"check_unsat_3"(get_ml_prog_state()))
+    [ordv; f1v; f2v]
+    (STDIO fs)
+    (POSTv uv. &UNIT_TYPE () uv *
+    SEP_EXISTS out err.
+      STDIO (add_stdout (add_stderr fs err) out) *
+      &(check_unsat_3_sem fs ord f1 out))
+Proof
+  rw[check_unsat_3_sem_def]>>
+  xcf "check_unsat_3" (get_ml_prog_state ())>>
+  reverse (Cases_on `STD_streams fs`) >- (fs [TextIOProofTheory.STDIO_def] \\ xpull) >>
+  xlet_autop>>
+  pop_assum mp_tac>>
+  TOP_CASE_TAC
+  >- (
+    simp[SUM_TYPE_def]>>rw[]>>
+    xmatch>>
+    xapp_spec output_stderr_spec \\ xsimpl>>
+    asm_exists_tac>>xsimpl>>
+    qexists_tac`emp`>>xsimpl>>
+    qexists_tac`fs`>>xsimpl>>
+    rw[]>>
+    qexists_tac`err`>>xsimpl>>rw[]>>
+    fs[STD_streams_add_stderr, STD_streams_stdout,add_stdo_nil]>>
+    xsimpl)>>
+  simp[SUM_TYPE_def]>>rw[]>>
+  xmatch>>
+  drule check_unsat_mo_top_norm_spec>>
+  strip_tac>>
+  xlet_auto
+  >- (
+    xsimpl>>
+    fs[validArg_def]>>
+    metis_tac[])>>
+  xlet_autop>>
+  every_case_tac>>gvs[SUM_TYPE_def]
+  >- (
+    fs[map_front_to_string_def,SUM_TYPE_def]>>
+    xmatch>>
+    xapp_spec output_stderr_spec \\ xsimpl>>
+    asm_exists_tac>>xsimpl>>
+    qexists_tac`emp`>>xsimpl>>
+    qexists_tac`fs`>>xsimpl>>
+    rw[]>>
+    qexists_tac`«»`>>
+    rename1`add_stderr _ err`>>
+    qexists_tac`err`>>xsimpl>>rw[]>>
+    fs[STD_streams_add_stderr, STD_streams_stdout,add_stdo_nil]>>
+    xsimpl)>>
+  fs[map_front_to_string_def,SUM_TYPE_def]>>
+  xmatch>>
+  xapp>>xsimpl>>
+  asm_exists_tac>>simp[]>>
+  qexists_tac`emp`>>qexists_tac`fs`>>xsimpl>>
+  rw[]>>
+  rename1`vomap_TYPE (print_front_str ord vs) _`>>
+  qexists_tac`print_front_str ord vs`>>simp[]>>
+  qexists_tac`«»`>>
+  simp[STD_streams_stderr,add_stdo_nil]>>
+  xsimpl>>
+  rw[]>>
+  rename1`get_mo_fml _ _ = SOME mprob`>>
+  qexists_tac`FST mprob`>>qexists_tac`SND mprob`>>qexists_tac`vs`>>
+  simp[]
+QED
+
+Definition usage_string_def:
+  usage_string = «Usage: cake_pb_mo <ordering: pareto> <OPB file> <optional: PB proof file>\n»
+End
+
+val r = translate usage_string_def;
+
+Quote add_cakeml:
+  fun main u =
+  case CommandLine.arguments () of
+    [ords,f1] =>
+      (case parse_mo_ord ords of
+        None => TextIO.output TextIO.stdErr (mk_usage_string usage_string)
+      | Some ord => check_unsat_2 f1)
+  | [ords,f1,f2] =>
+      (case parse_mo_ord ords of
+        None => TextIO.output TextIO.stdErr (mk_usage_string usage_string)
+      | Some ord => check_unsat_3 ord f1 f2)
+  | _ => TextIO.output TextIO.stdErr (mk_usage_string usage_string)
+End
+
+Definition main_sem_def:
+  main_sem fs cl out =
+  if LENGTH cl = 3 then
+    (case parse_mo_ord (EL 1 cl) of
+      NONE => out = «»
+    | SOME ord => check_unsat_2_sem fs (EL 2 cl) out)
+  else if LENGTH cl = 4 then
+    (case parse_mo_ord (EL 1 cl) of
+      NONE => out = «»
+    | SOME ord => check_unsat_3_sem fs ord (EL 2 cl) out)
+  else out = «»
+End
+
+Theorem STDIO_refl:
+  STDIO A ==>>
+  STDIO A * GC
+Proof
+  xsimpl
+QED
+
+Theorem main_spec:
+  hasFreeFD fs
+  ⇒
+  app (p:'ffi ffi_proj) ^(fetch_v"main"(get_ml_prog_state()))
+    [Conv NONE []]
+    (COMMANDLINE cl * STDIO fs)
+    (POSTv uv. &UNIT_TYPE () uv *
+    COMMANDLINE cl *
+    SEP_EXISTS out err.
+      STDIO (add_stdout (add_stderr fs err) out) *
+      &(main_sem fs cl out))
+Proof
+  rw[main_sem_def]>>
+  xcf"main"(get_ml_prog_state())>>
+  reverse (Cases_on `STD_streams fs`) >- (fs [TextIOProofTheory.STDIO_def] \\ xpull) >>
+  reverse(Cases_on`wfcl cl`) >- (fs[COMMANDLINE_def] \\ xpull)>>
+  rpt xlet_autop >>
+  Cases_on `cl` >- fs[wfcl_def] >>
+  rename1`wfcl (_::args)`>>
+  Cases_on`args`>>fs[LIST_TYPE_def]
+  >- (
+    xmatch>>
+    assume_tac (theorem "usage_string_v_thm")>>
+    xlet_autop>>
+    xapp_spec output_stderr_spec \\ xsimpl>>
+    rename1`COMMANDLINE cl`>>
+    qexists_tac`COMMANDLINE cl`>>xsimpl>>
+    qexists_tac `mk_usage_string usage_string` >>
+    simp [] >>
+    qexists_tac`fs`>>xsimpl>>
+    rw[]>>
+    fs[STD_streams_add_stderr, STD_streams_stdout,add_stdo_nil]>>
+    metis_tac[STDIO_refl])>>
+  rename1`wfcl (_::ords::args)`>>
+  Cases_on`args`>>fs[LIST_TYPE_def]
+  >- (
+    xmatch>>
+    assume_tac (theorem "usage_string_v_thm")>>
+    xlet_autop>>
+    xapp_spec output_stderr_spec \\ xsimpl>>
+    rename1`COMMANDLINE cl`>>
+    qexists_tac`COMMANDLINE cl`>>xsimpl>>
+    qexists_tac `mk_usage_string usage_string` >>
+    simp [] >>
+    qexists_tac`fs`>>xsimpl>>
+    rw[]>>
+    fs[STD_streams_add_stderr, STD_streams_stdout,add_stdo_nil]>>
+    metis_tac[STDIO_refl])>>
+  rename1`wfcl (_::ords::f1::args)`>>
+  Cases_on`args`>>fs[LIST_TYPE_def]
+  >- (
+    xmatch>>
+    xlet_autop>>
+    Cases_on`parse_mo_ord ords`>>fs[OPTION_TYPE_def]>>
+    xmatch
+    >- (
+      assume_tac (theorem "usage_string_v_thm")>>
+      xlet_autop>>
+      xapp_spec output_stderr_spec \\ xsimpl>>
+      rename1`COMMANDLINE cl`>>
+      qexists_tac`COMMANDLINE cl`>>xsimpl>>
+      qexists_tac `mk_usage_string usage_string` >>
+      simp [] >>
+      qexists_tac`fs`>>xsimpl>>
+      rw[]>>
+      fs[STD_streams_add_stderr, STD_streams_stdout,add_stdo_nil]>>
+      metis_tac[STDIO_refl])>>
+    xapp>>rw[]>>
+    rpt(first_x_assum (irule_at Any)>>xsimpl)>>
+    fs[wfcl_def]>>
+    rw[]>>metis_tac[STDIO_refl])>>
+  rename1`wfcl (_::ords::f1::f2::args)`>>
+  Cases_on`args`>>fs[LIST_TYPE_def]
+  >- (
+    xmatch>>
+    xlet_autop>>
+    Cases_on`parse_mo_ord ords`>>fs[OPTION_TYPE_def]>>
+    xmatch
+    >- (
+      assume_tac (theorem "usage_string_v_thm")>>
+      xlet_autop>>
+      xapp_spec output_stderr_spec \\ xsimpl>>
+      rename1`COMMANDLINE cl`>>
+      qexists_tac`COMMANDLINE cl`>>xsimpl>>
+      qexists_tac `mk_usage_string usage_string` >>
+      simp [] >>
+      qexists_tac`fs`>>xsimpl>>
+      rw[]>>
+      fs[STD_streams_add_stderr, STD_streams_stdout,add_stdo_nil]>>
+      metis_tac[STDIO_refl])>>
+    xapp>>rw[]>>
+    rpt(first_x_assum (irule_at Any)>>xsimpl)>>
+    fs[wfcl_def]>>
+    rw[]>>metis_tac[STDIO_refl])>>
+  xmatch>>
+  assume_tac (theorem "usage_string_v_thm")>>
+  xlet_autop>>
+  xapp_spec output_stderr_spec \\ xsimpl>>
+  rename1`COMMANDLINE cl`>>
+  qexists_tac`COMMANDLINE cl`>>xsimpl>>
+  qexists_tac `mk_usage_string usage_string` >>
+  simp [] >>
+  qexists_tac`fs`>>xsimpl>>
+  rw[]>>
+  fs[STD_streams_add_stderr, STD_streams_stdout,add_stdo_nil]>>
+  metis_tac[STDIO_refl]
+QED
+
+Theorem main_whole_prog_spec2:
+   hasFreeFD fs ⇒
+   whole_prog_spec2 main_v cl fs NONE
+     (λfs'. ∃out err.
+        fs' = add_stdout (add_stderr fs err) out ∧
+        main_sem fs cl out)
+Proof
+  rw[basis_ffiTheory.whole_prog_spec2_def]
+  \\ match_mp_tac (MP_CANON (DISCH_ALL (MATCH_MP app_wgframe (UNDISCH main_spec))))
+  \\ xsimpl
+  \\ rw[PULL_EXISTS]
+  \\ qexists_tac`add_stdout (add_stderr fs x') x`
+  \\ xsimpl
+  \\ qexists_tac`x`
+  \\ qexists_tac`x'`
+  \\ xsimpl
+  \\ simp[GSYM add_stdo_with_numchars,with_same_numchars]
+QED
+
+Theorem main_semantics =
+  prove_sem_thm "main"
+                "main_prog"
+                main_whole_prog_spec2;
